floyd/client_lemmas.v
@@ -913,13 +913,13 @@ end.
 
 Lemma Vint_inj: forall x y, Vint x = Vint y -> x=y.
 Proof. congruence. Qed.
-Lemma eval_cast_id:
+Lemma sem_cast_id:
   forall Delta rho,
       tc_environ Delta rho ->
   forall t1 t3 id,
   Cop.classify_cast t1 t3 = Cop.cast_case_neutral ->
   match (temp_types Delta)!id with Some (Tpointer _ _, true) => true | _ => false end = true ->
-  eval_cast t1 t3 (eval_id id rho) = eval_id id rho.
+  force_val (sem_cast t1 t3 (eval_id id rho)) = eval_id id rho.
 Proof.
 intros.
  revert H1; case_eq ((temp_types Delta) ! id); intros; try discriminate.
@@ -936,39 +936,116 @@ intros.
   try (destruct i0; inv H3); try (destruct i1; inv H2); try reflexivity.
 Qed.
 
-Lemma eval_cast_pointer2':
+Lemma sem_cast_pointer2':
   forall (v : val) (t1 t2: type),
   match t1 with Tpointer _ _ | Tint I32 _ _ => True | _ => False end ->
   match t2 with Tpointer _ _ | Tint I32 _ _ => True | _ => False end ->
-  is_pointer_or_null v -> eval_cast t1 t2 v = v.
+  is_pointer_or_null v -> force_val (sem_cast t1 t2 v) = v.
 Proof.
 intros.
-unfold eval_cast, classify_cast.
+unfold sem_cast, classify_cast.
 subst.
 destruct t1; try contradiction; try destruct i; try contradiction; simpl; auto;
 destruct t2; try contradiction; try destruct i; try contradiction; simpl; auto;
 destruct v; inv H1; simpl; auto.
 Qed.
 
-Hint Rewrite eval_cast_pointer2' using (try apply I; try assumption; reflexivity) : norm.
+Hint Rewrite sem_cast_pointer2' using (try apply I; try assumption; reflexivity) : norm.
 
 Lemma typecheck_val_eq:
   forall v t, (typecheck_val v t = true) = tc_val t v.
 Proof. intros. rewrite tc_val_eq. reflexivity. Qed.
 Hint Rewrite typecheck_val_eq : norm.
 
-Lemma eval_cast_pointer2: 
+Lemma sem_cast_pointer2: 
   forall v t1 t2 t3 t1' t2',
    t1' = Tpointer t1 noattr ->
    t2' = Tpointer t2 noattr ->
    tc_val (Tpointer t3 noattr) v ->
-   eval_cast t1' t2' v = v.
+   force_val (sem_cast t1' t2' v) = v.
 Proof.
 intros.
 subst.
 hnf in H1. destruct v; inv H1; reflexivity.
 Qed.
 
+Lemma force_eval_var_int_ptr :
+forall Delta rho i t,
+tc_environ Delta rho ->
+tc_lvalue Delta (Evar i t) rho -> 
+          force_val
+            match eval_var i t rho with
+            | Vundef => None
+            | Vint _ => Some (eval_var i t rho)
+            | Vlong _ => None
+            | Vfloat _ => None
+            | Vptr _ _ => Some (eval_var i t rho)
+            end = eval_var i t rho.
+Proof.
+intros.
+ pose proof (expr_lemmas.typecheck_lvalue_sound _ _ _ H H0).
+ simpl in H1.
+ destruct (eval_var i t rho); inv H1; simpl; auto.
+Qed.
+
+
+Lemma force_eval_var_int_ptr':
+ forall i t rho,
+  (exists Delta,
+    tc_environ Delta rho /\  tc_lvalue Delta (Evar i t) rho) ->
+  force_val
+            match eval_var i t rho with
+            | Vundef => None
+            | Vint _ => Some (eval_var i t rho)
+            | Vlong _ => None
+            | Vfloat _ => None
+            | Vptr _ _ => Some (eval_var i t rho)
+            end = eval_var i t rho.
+Proof.
+intros.
+ destruct H as [Delta [? ?]];
+ eapply force_eval_var_int_ptr; eauto.
+Qed.
+
+Hint Rewrite force_eval_var_int_ptr' using 
+   match goal with Delta := _ : tycontext |- _ => 
+       exists Delta; split; hnf; solve [auto]
+   end : norm.     
+
+Lemma is_pointer_or_null_force_int_ptr:
+   forall v, is_pointer_or_null v -> (force_val
+        match v with
+        | Vundef => None
+        | Vint _ => Some v
+        | Vlong _ => None
+        | Vfloat _ => None
+        | Vptr _ _ => Some v end) = v.
+Proof.
+intros. destruct v; inv H; reflexivity.
+Qed.
+Hint Rewrite is_pointer_or_null_force_int_ptr using assumption : norm.
+
+
+Lemma is_pointer_or_null_force_int_ptr2:
+   forall v, is_pointer_or_null (force_val
+        match v with
+        | Vundef => None
+        | Vint _ => Some v
+        | Vlong _ => None
+        | Vfloat _ => None
+        | Vptr _ _ => Some v end) -> (force_val
+        match v with
+        | Vundef => None
+        | Vint _ => Some v
+        | Vlong _ => None
+        | Vfloat _ => None
+        | Vptr _ _ => Some v end) = v.
+Proof.
+intros. destruct v; inv H; reflexivity.
+Qed.
+
+Hint Rewrite is_pointer_or_null_force_int_ptr2 using assumption : norm.
+(*
 Lemma eval_cast_neutral_var:
  forall Delta rho, 
   tc_environ Delta rho -> 
@@ -981,7 +1058,6 @@ intros.
  simpl in H1.
  destruct (eval_var i t rho); inv H1; simpl; auto.
 Qed.
-
   
 Lemma eval_cast_neutral_var':
  forall i t rho,
@@ -1015,6 +1091,7 @@ intros. destruct v; inv H; reflexivity.
 Qed.
 Hint Rewrite eval_cast_neutral_is_pointer_or_null using assumption : norm.
 
+
 Lemma is_pointer_or_null_eval_cast_neutral:
   forall v, is_pointer_or_null (eval_cast_neutral v) = is_pointer_or_null v.
 Proof. destruct v; reflexivity. Qed.
@@ -1028,7 +1105,7 @@ Qed.
 Hint Rewrite eval_cast_neutral_isptr using assumption : norm.
 
 Ltac eval_cast_simpl :=
-    try (unfold eval_cast; simpl Cop.classify_cast; cbv iota);
+    try (try unfold eval_cast; simpl Cop.classify_cast; cbv iota);
      try match goal with H: tc_environ ?Delta ?rho |- _ =>
        repeat first [rewrite (eval_cast_neutral_var Delta rho H) by reflexivity
                | rewrite eval_cast_neutral_isptr by auto
@@ -1036,6 +1113,19 @@ Ltac eval_cast_simpl :=
                | erewrite eval_cast_pointer2; [ | | | eassumption ]; [ | reflexivity | reflexivity ]
                ]
      end.
+
+(*
+Ltac eval_cast_simpl :=
+     try match goal with H: tc_environ ?Delta ?rho |- _ =>
+       repeat first [rewrite (eval_cast_var Delta rho H); [ | reflexivity | hnf; simpl; normalize ]
+               | rewrite (eval_cast_id Delta rho H); [ | reflexivity | reflexivity ]
+               | rewrite eval_cast_int; [ | assumption]
+               | erewrite eval_cast_pointer2; [ | | | eassumption ]; [ | reflexivity | reflexivity ]
+               ]
+     end.
+*)
+*)
+
 
 Lemma fold_right_nil: forall {A B} (f: A -> B -> B) (z: B),
    fold_right f z nil = z.
@@ -1069,12 +1159,12 @@ Arguments ret_type !Delta /.
 Ltac unfold_for_go_lower :=
   cbv delta [PROPx LOCALx SEPx
                        eval_exprlist eval_expr eval_lvalue cast_expropt 
-                       eval_cast eval_binop eval_unop
+                       sem_cast eval_binop eval_unop
                       tc_expropt tc_expr tc_lvalue 
                       typecheck_expr typecheck_lvalue
                       function_body_ret_assert 
                       make_args' bind_ret get_result1 retval
-                      eval_cast classify_cast
+                       classify_cast
                       denote_tc_assert
     liftx LiftEnviron Tarrow Tend lift_S lift_T
     lift_prod lift_last lifted lift_uncurry_open lift_curry 
